Move identifiers to identifiers.v

theories/L6_PCPS/uncurry_correct.v
@@ -567,497 +567,6 @@ Section uncurry_correct.
   Definition fresh_copies (s : Ensemble var) (l : list var) : Prop
     := Disjoint _ s (FromList l) /\ NoDup l.
 
-  (* ------------------------------ facts about variables ------------------------------ *)
-
-  (* all the used variables in an expression *)
-  Definition used_vars (e : exp) : Ensemble var := bound_var e :|: occurs_free e.
-  Definition used_vars_fundefs (fds : fundefs) : Ensemble var
-    := bound_var_fundefs fds :|: occurs_free_fundefs fds.
-  Definition used_vars_ctx (c : exp_ctx) : Ensemble var
-    := bound_var_ctx c :|: occurs_free_ctx c.
-  Definition used_vars_fundefs_ctx (f : fundefs_ctx) : Ensemble var
-    := bound_var_fundefs_ctx f :|: occurs_free_fundefs_ctx f.
-
-  Lemma Decidable_Empty_set : forall A, Decidable (Empty_set A).
-  Proof. intros; constructor; intros; right; now inversion 1. Qed.
-
-  Lemma used_vars_dec: forall e, Decidable (used_vars e).
-  Proof.
-    intros e.
-    apply Decidable_Union.
-    apply bound_var_dec.
-    apply Decidable_occurs_free.
-  Qed.
-
-  Lemma used_vars_fundefs_dec: forall fds, Decidable (used_vars_fundefs fds).
-  Proof.
-    intros fds.
-    apply Decidable_Union.
-    apply bound_var_fundefs_dec.
-    apply Decidable_occurs_free_fundefs.
-  Qed.
-
-  Lemma used_vars_ctx_dec: forall e, Decidable (used_vars_ctx e).
-  Proof.
-    intros e.
-    apply Decidable_Union.
-    apply bound_var_ctx_dec.
-    apply Decidable_occurs_free_ctx.
-  Qed.
-
-  Lemma used_vars_fundefs_ctx_dec: forall fds, Decidable (used_vars_fundefs_ctx fds).
-  Proof.
-    intros fds.
-    apply Decidable_Union.
-    apply bound_var_fundefs_ctx_dec.
-    apply Decidable_occurs_free_fundefs_ctx.
-  Qed.
-
-  (* -------------------------------------------------------------------------------- *)
-
-  Lemma Decidable_not_not : forall {A} (S : Ensemble A),
-    Decidable S -> forall a,
-    ~ ~ In _ S a <-> In _ S a.
-  Proof.
-    intros A S HS a;
-    destruct HS as [HS];
-    specialize HS with (x := a);
-    destruct HS as [HS|HS];
-    split; easy.
-  Qed.
-
-  Lemma occurs_in_vars_correct : forall a l, occurs_in_vars a l = true <-> List.In a l.
-  Proof.
-    induction l; [firstorder|].
-    destruct (Pos.eqb_spec a a0); subst.
-    simpl; rewrite Pos.eqb_refl; simpl; split; intros; [now left|easy].
-    simpl; rewrite <- Pos.eqb_neq in n; unfold eq_var; rewrite n; simpl.
-    rewrite IHl.
-    split; [intros H; now right|intros [contra|H]]; [|assumption].
-    rewrite Pos.eqb_neq in n; congruence.
-  Qed.
-
-  Corollary occurs_in_vars_correct_neq : forall a l, occurs_in_vars a l = false <-> ~ List.In a l.
-  Proof.
-    assert (forall a, a = false <-> ~ (a = true)). {
-      split; intros Ha.
-      - intros Hcontra; congruence.
-      - destruct a; [congruence|reflexivity].
-    } 
-    intros; rewrite H.
-    apply not_iff_compat.
-    apply occurs_in_vars_correct.
-  Qed.
-
-  Lemma Union_demorgan : forall {A} (l r : Ensemble A) a,
-    ~ In _ (l :|: r) a <-> ~ In _ l a /\ ~ In _ r a.
-  Proof.
-    split; intros.
-    - split; intros contra; contradiction H.
-      now left. now right.
-    - destruct H. intros contra. inv contra; congruence.
-  Qed.
-
-  (*
-  Lemma Intersection_demorgan : forall {A} (l r : Ensemble A) a,
-    ~ In _ (l :&: r) a <-> ~ In _ l a \/ ~ In _ r a.
-  Proof.
-    split; intros.
-    - split; intros contra; contradiction H.
-      now left. now right.
-    - destruct H. intros contra. inv contra; congruence.
-  Qed.
-*)
-  Lemma negb_not : forall a b, a = negb b <-> a <> b.
-  Proof. destruct a; destruct b; firstorder. Qed.
-
-  Lemma Disjoint_Singleton_In : forall A S a,
-    Decidable S -> Disjoint A S [set a] <-> ~ In _ S a.
-  Proof.
-    split; intros H.
-    - inv H; specialize H0 with (x := a).
-      destruct X; destruct (Dec a); [|easy].
-      contradiction H0; constructor; easy.
-    - constructor.
-      intros x contra; inv contra.
-      now inv H1.
-  Qed.
-
-  Lemma not_Disjoint_Singleton_In : forall A S a,
-    Decidable S -> ~ Disjoint A S [set a] <-> In _ S a.
-  Proof.
-    split; [intros H|inversion 2; eapply H0; eauto].
-    destruct X; destruct (Dec a); [easy|].
-    contradiction H; constructor; intros.
-    intros contra; destruct contra.
-    inv H1.
-    contradiction.
-  Qed.
-
-  Lemma find_def_is_Some_occurs_free_fundefs : forall f fds t xs e a,
-    find_def f fds = Some (t, xs, e) ->
-    occurs_free e a ->
-    ~ List.In a xs ->
-    ~ name_in_fundefs fds a ->
-    occurs_free_fundefs fds a.
-  Proof.
-    induction fds; simpl; intros; [|now contradiction H2].
-    destruct (M.elt_eq f v); [subst; inv H|].
-    - constructor; auto; intros contra; subst; contradiction H2; [now left|now right].
-    - apply Free_Fcons2; [|intros contra; subst; contradiction H2; now left].
-      eapply IHfds; eauto.
-      intros contra; subst; contradiction H2; now right.
-  Qed.
-
-  Ltac split_var_eq a b :=
-    destruct (PS.Raw.MX.eq_dec a b).
-
-  Ltac split_var_in_list a l :=
-    destruct (in_dec PS.Raw.MX.eq_dec a l).
-
-  Ltac split_var_in_fundefs a fds Hfds :=
-    destruct (Decidable_name_in_fundefs fds) as [Hfds]; destruct (Hfds a).
-
-  Local Ltac solve_bound_cases a v l := 
-    split_var_eq a v; split_var_in_list a l;
-    [ right; now constructor
-    | left; subst a; constructor
-    | right; now constructor
-    | right].
-
-  Hint Resolve used_vars_dec : Decidable_DB.
-  Hint Resolve used_vars_fundefs_dec : Decidable_DB.
-  Hint Resolve bound_var_dec : Decidable_DB.
-  Hint Resolve bound_var_fundefs_dec : Decidable_DB.
-  Hint Resolve Decidable_occurs_free : Decidable_DB.
-  Hint Resolve Decidable_occurs_free_fundefs : Decidable_DB.
-  Hint Resolve Decidable_name_in_fundefs : Decidable_DB.
-  Hint Resolve Decidable_Empty_set : Decidable_DB.
-  Hint Resolve Decidable_Union : Decidable_DB.
-  Hint Resolve Decidable_Intersection : Decidable_DB.
-  Hint Resolve Decidable_Setminus : Decidable_DB.
-  Hint Resolve Decidable_singleton_var : Decidable_DB.
-  Hint Resolve Decidable_FromList : Decidable_DB.
-  Hint Resolve Decidable_occurs_free : Decidable_DB.
-
-  Local Ltac simplify_boolean_exprs := 
-    simpl in *;
-    repeat rewrite orb_false_r in *;
-    repeat rewrite orb_true_r in *;
-    simpl in *.
-
-  Local Ltac rewrite_trivial_iffs :=
-    repeat match goal with
-    | [ Heq : ?a <-> ?b, Ha : ?a |- _ ] => (assert b by now rewrite <- Heq); clear Heq
-    | [ Heq : ?a <-> ?b |- ?a ] => rewrite Heq
-    | [ Heq : true = false <-> ~ In var ?S ?a |- _ ] =>
-        apply not_iff_compat in Heq;
-        rewrite <- negb_not in Heq;
-        (rewrite Decidable_not_not in Heq; [|auto]);
-        (assert (In var S a) by now rewrite <- Heq); clear Heq
-    | [ Heq : false = false <-> In var ?S ?a |- _ ] =>
-        (assert (In var S a) by now rewrite <- Heq); clear Heq
-    | [ Heq : false = false <-> ~ In var ?S ?a |- _ ] => 
-        (assert (~ In var S a) by now rewrite <- Heq); clear Heq
-    end.
-
-  Local Ltac eliminate_singleton_disjoints :=
-    repeat match goal with
-    | [ Hin : _ = _ <-> Disjoint _ _ [set _] |- _ ] =>
-        rewrite Disjoint_Singleton_In in Hin; [|auto]
-    | [ Hin : _ = _ <-> ~ Disjoint _ _ [set _] |- _ ] =>
-        rewrite not_Disjoint_Singleton_In in Hin; [|auto]
-    | [ Hin : Disjoint _ _ [set _] |- _ ] =>
-        rewrite Disjoint_Singleton_In in Hin; [|auto]
-    | [ Hin : ~ Disjoint _ _ [set _] |- _ ] =>
-        rewrite not_Disjoint_Singleton_In in Hin; [|auto]
-    end;
-    try (rewrite Disjoint_Singleton_In; [|auto]);
-    try (rewrite not_Disjoint_Singleton_In; [|auto]).
-
-  Local Ltac demorgan_not_used_vars :=
-    repeat match goal with
-    | [ Hin : ~ In var (used_vars _) _ |- _ ] =>
-        unfold used_vars in Hin;
-        rewrite Union_demorgan in Hin;
-        destruct Hin
-    | [ Hin : ~ In var (used_vars_fundefs _) _ |- _ ] =>
-        unfold used_vars_fundefs in Hin;
-        rewrite Union_demorgan in Hin;
-        destruct Hin
-    end.
-
-  Local Ltac cleanup :=
-    try (rewrite occurs_in_vars_correct in *);
-    try (rewrite occurs_in_vars_correct_neq in *);
-    simplify_boolean_exprs;
-    eliminate_singleton_disjoints;
-    rewrite_trivial_iffs;
-    demorgan_not_used_vars.
-
-  Local Ltac super_destruct e Hvar :=
-    destruct e eqn:Hvar;
-    simpl in *;
-    try rewrite Hvar in *;
-    try (rewrite Pos.eqb_eq in Hvar; subst);
-    try (rewrite Pos.eqb_neq in Hvar);
-    cleanup;
-    try congruence.
-
-  Lemma Ensemble_iff_In_iff : forall {A} (S1 S2 : _ A),
-    (S1 <--> S2) <-> (forall a, In _ S1 a <-> In _ S2 a).
-  Proof.
-    split; intros.
-    now rewrite H.
-    unfold Same_set, Included.
-    firstorder.
-  Qed.
-
-  Lemma not_In_Setminus : forall {A} S1 S2 x, (In _ (S1 \\ S2) x <-> In _ S1 x /\ ~ In A S2 x).
-  Proof. split; intros; [inversion H|constructor]; tauto. Qed.
-
-  Lemma In_Singleton : forall A x y, In A [set x] y <-> x = y.
-  Proof. split; intros; [now inversion H|now subst]. Qed.
-
-  Lemma not_In_Singleton : forall A x y, ~ In A [set x] y <-> x <> y.
-  Proof. split; intros; intros oops; apply H; [now subst|now inversion oops]. Qed.
-
-  Lemma In_Empty_set : forall A x, In A (Empty_set A) x <-> False.
-  Proof. split; intros; inversion H. Qed.
-
-  Lemma not_In_Empty_set : forall A x, ~ In A (Empty_set A) x <-> True.
-  Proof. split; intros; auto; inversion 1. Qed.
-
-  Lemma eq_var_iff_Singleton_l : forall b a, eq_var a b = true <-> In _ [set a] b.
-  Proof.
-    split; intros H; destruct (eq_var a b) eqn:Heq; try congruence.
-    rewrite Pos.eqb_eq in Heq; now subst.
-    rewrite Pos.eqb_neq in Heq; contradiction Heq; now inv H.
-  Qed.
-
-  Lemma eq_var_iff_Singleton_r : forall a b, eq_var a b = true <-> In _ [set b] a.
-  Proof.
-    split; intros H; destruct (eq_var a b) eqn:Heq; try congruence.
-    rewrite Pos.eqb_eq in Heq; now subst.
-    rewrite Pos.eqb_neq in Heq; contradiction Heq; now inv H.
-  Qed.
-
-  Lemma In_or_Iff_Union : forall {A} (a : A) S1 S2,
-    In _ (S1 :|: S2) a <-> In _ S1 a \/ In _ S2 a.
-  Proof. split; intros; destruct H; auto. Qed.
-
-  Local Ltac inv_all :=
-    repeat match goal with
-    | [ H : In var _ _ |- _ ] => inv H
-    | [ H : List.In _ _ |- _ ] => inv H
-    | [ H : (_, _) = (_, _) |- _ ] => inv H
-    end;
-    eauto with Ensembles_DB.
-
-  Lemma occurs_in_exp_correct_mut : forall x,
-    (forall e, (fun e => occurs_in_exp x e = false <-> Disjoint _ (used_vars e) [set x]) e) /\
-    (forall f, (fun f => occurs_in_fundefs x f = false <-> Disjoint _ (used_vars_fundefs f) [set x]) f).
-  Proof.
-    intros x.
-    apply exp_def_mutual_ind;
-    (* Rewrite by IH and translate everything to FOL *)
-    simpl; intros;
-    repeat match goal with H : ?lhs = false <-> Disjoint _ _ _ |- _ => revert H end;
-    repeat rewrite orb_false_iff;
-    repeat match goal with |- context [eq_var ?x ?y = false] => rewrite (Pos.eqb_neq x y) end;
-    repeat match goal with |- context [eq_var ?x ?y = true] => rewrite (Pos.eqb_eq x y) end;
-    repeat rewrite occurs_in_vars_correct;
-    repeat rewrite occurs_in_vars_correct_neq;
-    (* Normalize used_vars *)
-    unfold used_vars; unfold used_vars_fundefs; repeat rewrite Union_demorgan;
-    repeat normalize_bound_var; repeat normalize_occurs_free;
-    (* Normalize expressions involving In and solve with tauto/intuition *)
-    repeat eliminate_singleton_disjoints;
-    repeat (rewrite Union_demorgan
-     || rewrite not_In_Setminus
-     || rewrite In_Singleton
-     || rewrite not_In_Singleton
-     || rewrite In_Empty_set
-     || rewrite not_In_Empty_set);
-    (* Explain that name_in_fundefs S ⊆ bound_var_fundefs S *)
-    repeat lazymatch goal with
-    | H : In _ (name_in_fundefs ?S) ?x -> In _ (bound_var_fundefs ?S) ?x |-
-      context [In _ (name_in_fundefs ?S) ?x] => fail
-    | |- context [In _ (name_in_fundefs ?S) ?x] => 
-      assert (In _ (name_in_fundefs S) x -> In _ (bound_var_fundefs S) x)
-        by apply name_in_fundefs_bound_var_fundefs
-    end;
-    try match goal with |- Decidable _ => eauto 20 with Decidable_DB end;
-    solve [tauto|intuition congruence|firstorder|eauto with Ensembles_DB].
-  Qed.
-
-  Corollary occurs_in_exp_correct : forall x e,
-    occurs_in_exp x e = false <-> Disjoint _ (used_vars e) [set x].
-  Proof. apply occurs_in_exp_correct_mut. Qed.
-
-  Corollary occurs_in_fundefs_correct : forall x f,
-    occurs_in_fundefs x f = false <-> Disjoint _ (used_vars_fundefs f) [set x].
-  Proof. apply occurs_in_exp_correct_mut. Qed.
-
-  Corollary occurs_in_exp_iff_used_vars : forall e a,
-    occurs_in_exp a e = true <-> In _ (used_vars e) a.
-  Proof.
-    intros.
-    rewrite <- Decidable_not_not by auto with Decidable_DB; auto.
-    replace true with (negb false); auto.
-    rewrite negb_not.
-    apply not_iff_compat.
-    rewrite <- Disjoint_Singleton_In by auto with Decidable_DB; auto.
-    apply occurs_in_exp_correct.
-  Qed.
-
-  Corollary not_occurs_in_exp_iff_used_vars : forall e a,
-    occurs_in_exp a e = false <-> ~ In _ (used_vars e) a.
-  Proof. intros. rewrite <- Disjoint_Singleton_In; auto with Decidable_DB.
-         apply occurs_in_exp_correct. Qed.
-
-  Corollary occurs_in_fundefs_iff_used_vars_fundefs : forall e a,
-    occurs_in_fundefs a e = true <-> In _ (used_vars_fundefs e) a.
-  Proof with auto with Decidable_DB.
-    intros.
-    rewrite <- Decidable_not_not...
-    replace true with (negb false); auto.
-    rewrite negb_not.
-    apply not_iff_compat.
-    rewrite <- Disjoint_Singleton_In...
-    apply occurs_in_fundefs_correct.
-  Qed.
-
-  Corollary not_occurs_in_fundefs_iff_used_vars_fundefs : forall e a,
-    occurs_in_fundefs a e = false <-> ~ In _ (used_vars_fundefs e) a.
-  Proof with auto with Decidable_DB.
-    intros. rewrite <- Disjoint_Singleton_In...
-    apply occurs_in_fundefs_correct.
-  Qed.
-
-  Ltac translate_used_vars_to_firstorder a :=
-    repeat (
-      repeat rewrite <- occurs_in_exp_iff_used_vars in *; simpl in *;
-      repeat rewrite <- occurs_in_fundefs_iff_used_vars_fundefs in *; simpl in *;
-      repeat rewrite orb_true_iff in *;
-      repeat rewrite (eq_var_iff_Singleton_r a) in *;
-      repeat rewrite (eq_var_iff_Singleton_l a) in *;
-      repeat rewrite occurs_in_vars_correct in *;
-      repeat rewrite occurs_in_exp_iff_used_vars in *;
-      repeat rewrite occurs_in_fundefs_iff_used_vars_fundefs in *;
-      repeat rewrite In_or_Iff_Union in *
-    ).
-
-  Local Ltac solve_used_vars_lemma :=
-    intros;
-    rewrite Ensemble_iff_In_iff; intros a;
-    translate_used_vars_to_firstorder a;
-    firstorder.
-
-  Lemma used_vars_Econstr : forall x c args e,
-    used_vars (Econstr x c args e) <--> x |: FromList args :|: used_vars e.
-  Proof. solve_used_vars_lemma. Qed.
-
-  Lemma used_vars_Ecase_nil : forall x,
-    used_vars (Ecase x []) <--> [set x].
-  Proof. solve_used_vars_lemma. Qed.
-
-  Lemma used_vars_Ecase_cons : forall x c e arms,
-    used_vars (Ecase x ((c, e) :: arms)) <--> used_vars e :|: used_vars (Ecase x arms).
-  Proof.
-    induction arms.
-    - intros; rewrite Ensemble_iff_In_iff; intros a.
-      translate_used_vars_to_firstorder a.
-      firstorder.
-    - destruct a; rewrite Ensemble_iff_In_iff; intros a.
-      translate_used_vars_to_firstorder a.
-      clear IHarms; firstorder.
-  Qed.
-
-  Lemma used_vars_Ecase_app : forall x l r,
-    used_vars (Ecase x (l ++ r)) <--> used_vars (Ecase x l) :|: used_vars (Ecase x r).
-  Proof.
-    destruct r as [| [c e] ces]; [rewrite app_nil_r; solve_used_vars_lemma|].
-    unfold used_vars.
-    rewrite bound_var_Ecase_app, occurs_free_Ecase_app.
-    normalize_bound_var; normalize_occurs_free.
-    split; intros a Ha; repeat match goal with H : In _ (_ :|: _) _ |- _ => destruct H end;
-    eauto with Ensembles_DB.
-  Qed.
-
-  Lemma used_vars_Eproj : forall x c n y e,
-    used_vars (Eproj x c n y e) <--> x |: (y |: used_vars e).
-  Proof. solve_used_vars_lemma. Qed.
-
-  Lemma used_vars_Efun : forall fds e,
-    used_vars (Efun fds e) <--> used_vars_fundefs fds :|: used_vars e.
-  Proof. solve_used_vars_lemma. Qed.
-
-  Lemma used_vars_Eletapp: forall x f ft ys e,
-    used_vars (Eletapp x f ft ys e) <--> x |: (f |: FromList ys :|: used_vars e).
-  Proof. solve_used_vars_lemma. Qed.
-
-  Lemma used_vars_Eapp: forall f t args,
-    used_vars (Eapp f t args) <--> f |: FromList args.
-  Proof. solve_used_vars_lemma. Qed.
-
-  Lemma used_vars_Eprim : forall x p args e,
-    used_vars (Eprim x p args e) <--> x |: FromList args :|: used_vars e.
-  Proof. solve_used_vars_lemma. Qed.
-
-  Lemma used_vars_Ehalt : forall x, used_vars (Ehalt x) <--> [set x].
-  Proof. solve_used_vars_lemma. Qed.
-
-  Lemma used_vars_Fcons : forall f t v e fds,
-    used_vars_fundefs (Fcons f t v e fds) <-->
-    f |: FromList v :|: used_vars e :|: used_vars_fundefs fds.
-  Proof. solve_used_vars_lemma. Qed.
-
-  Lemma used_vars_Fnil : used_vars_fundefs Fnil <--> Empty_set _.
-  Proof. solve_used_vars_lemma. Qed.
-
-  Ltac normalize_used_vars := 
-    match goal with
-    | |- context [ used_vars (Econstr _ _ _ _) ] => rewrite used_vars_Econstr
-    | |- context [ used_vars (Eproj _ _ _ _ _) ] => rewrite used_vars_Eproj
-    | |- context [ used_vars (Ecase _ []) ] => rewrite used_vars_Ecase_nil
-    | |- context [ used_vars (Ecase _ (_ :: _)) ] => rewrite used_vars_Ecase_cons
-    | |- context [ used_vars (Ecase _ (_ ++ _)) ] => rewrite used_vars_Ecase_app
-    | |- context [ used_vars (Efun _ _) ] => rewrite used_vars_Efun
-    | |- context [ used_vars (Eletapp _ _ _ _ _) ] => rewrite used_vars_Eletapp
-    | |- context [ used_vars (Eapp _ _ _) ] => rewrite used_vars_Eapp
-    | |- context [ used_vars (Eprim _ _ _ _) ] => rewrite used_vars_Eprim
-    | |- context [ used_vars (Ehalt _) ] => rewrite used_vars_Ehalt
-    | |- context [ used_vars_fundefs (Fcons _ _ _ _ _) ] => rewrite used_vars_Fcons
-    | |- context [ used_vars_fundefs Fnil ] => rewrite used_vars_Fnil
-    | [ H : context [ used_vars (Econstr _ _ _ _)         ] |- _ ] => rewrite used_vars_Econstr in H
-    | [ H : context [ used_vars (Eproj _ _ _ _ _)         ] |- _ ] => rewrite used_vars_Eproj in H
-    | [ H : context [ used_vars (Ecase _ [])              ] |- _ ] => rewrite used_vars_Ecase_nil in H
-    | [ H : context [ used_vars (Ecase _ (_ :: _))        ] |- _ ] => rewrite used_vars_Ecase_cons in H
-    | [ H : context [ used_vars (Efun _ _)                ] |- _ ] => rewrite used_vars_Efun in H
-    | [ H : context [ used_vars (Eapp _ _ _)              ] |- _ ] => rewrite used_vars_Eapp in H
-    | [ H : context [ used_vars (Eprim _ _ _ _)           ] |- _ ] => rewrite used_vars_Eprim in H
-    | [ H : context [ used_vars (Ehalt _)                 ] |- _ ] => rewrite used_vars_Ehalt in H
-    | [ H : context [ used_vars_fundefs (Fcons _ _ _ _ _) ] |- _ ] => rewrite used_vars_Fcons in H
-    | [ H : context [ used_vars_fundefs Fnil              ] |- _ ] => rewrite used_vars_Fnil in H
-    end.
-
-  Lemma used_vars_subset_mut :
-    (forall c, (fun c => forall e, used_vars e \subset used_vars (c |[ e ]|)) c) /\
-    (forall f, (fun f => forall e, used_vars e \subset used_vars_fundefs (f <[ e ]>)) f).
-  Proof with eauto with Ensembles_DB.
-    exp_fundefs_ctx_induction IHe IHf; simpl; try rename e into c;
-    try solve [easy|intros; repeat normalize_used_vars; eauto with Ensembles_DB].
-  Qed.
-
-  Corollary used_vars_subset : forall c e, 
-    used_vars e \subset used_vars (c |[ e ]|).
-  Proof. apply used_vars_subset_mut. Qed.
-
-  Corollary used_vars_subset_fundefs_ctx : forall f e, 
-    used_vars e \subset used_vars_fundefs (f <[ e ]>).
-  Proof. apply used_vars_subset_mut. Qed.
-
   (* "a small step" of uncurrying *)
   Inductive uncurry_step :
     exp -> (* original expression *)
@@ -1274,7 +783,7 @@ Section uncurry_correct.
     (HPost_appG : post_app_compat Post PostG)
     (HPost_letappG : post_letapp_compat cenv Post Post PostG)
     (HPost_letapp_OOTG : post_letapp_compat_OOT Post PostG)
-    (HPost_inclG : inclusion (exp * env * nat) Post PostG)
+    (HPost_inclG : inclusion _ Post PostG)
     (HPostG_Eapp : forall ge rho'' c1 f1 ft1 gv1 fv1 rho1'' c2,
       (* TODO add preconditions? *)
       PostG (ge, rho'', c1) (Eapp f1 ft1 (gv1 ++ fv1), rho1'', c2))
@@ -1288,6 +797,9 @@ Section uncurry_correct.
     (HPost_letapp_OOTGG : post_letapp_compat_OOT PostG PostG)
     (HPost_baseGG : post_base PostG)
     (HPostG_inclG : inclusion (exp * env * nat) PostG PostG).
+
+  Context (HcompPost : inclusion _ (comp Post Post) Post)
+          (HGPost' : inclusion _ PostG Post).  
 
   Lemma preord_val_fundefs : forall k rho rho1 fds f, 
     preord_env_P cenv Post (occurs_free_fundefs fds) k rho rho1 ->
@@ -2332,9 +1844,8 @@ Section uncurry_correct.
   Proof.
     induction arms; intros.
     - destruct arms1; inv H.
-    - destruct arms1; inv H; (constructor; [easy|]).
+    - destruct arms1; inv H; (constructor; [easy|]); auto.
       now apply List_util.Forall2_refl.
-      now apply IHarms.
   Qed.
 
   Lemma Union_Included_subst_l: forall (A : Type) (a b b' c : Ensemble A),
@@ -2343,57 +1854,23 @@ Section uncurry_correct.
 
   Lemma used_vars_fundefs_Fcons_Included: forall f t v e fds,
     used_vars_fundefs fds \subset used_vars_fundefs (Fcons f t v e fds).
-  Proof.
-    intros; intros x Hx.
-    destruct Hx; [left; now apply Bound_Fcons2|inv H].
-    split_var_eq x f; subst.
-    left; auto.
-    right; apply Free_Fcons2; auto.
-    split_var_eq x f; subst.
-    left; auto.
-    right; apply Free_Fcons2; auto.
-  Qed.
+  Proof. intros; normalize_used_vars; auto with Ensembles_DB. Qed.
 
   Lemma used_vars_Fcons_Included: forall f t v e fds,
     used_vars e \subset used_vars_fundefs (Fcons f t v e fds).
-  Proof.
-    intros; intros x Hx.
-    destruct Hx; [left; now apply Bound_Fcons3|].
-    split_var_eq x f; subst.
-    left; auto.
-    split_var_in_list x v; [left; constructor; auto|].
-    split_var_in_fundefs x fds Hfds.
-    left; apply Bound_Fcons2; now apply name_in_fundefs_bound_var_fundefs.
-    right; apply Free_Fcons1; auto.
-  Qed.
+  Proof. intros; normalize_used_vars; auto with Ensembles_DB. Qed.
 
   Lemma used_vars_Eprim_cons_Included: forall x p a args e,
     used_vars (Eprim x p args e) \subset used_vars (Eprim x p (a :: args) e).
-  Proof.
-    intros; intros y Hy; destruct Hy.
-    left. inv H; auto.
-    inv H; right.
-    constructor; now right.
-    apply Free_Eprim2; auto.
-  Qed.
+  Proof. intros; repeat normalize_used_vars; normalize_sets; auto with Ensembles_DB. Qed.
 
   Lemma used_vars_Efun_Included: forall fds e,
     used_vars e \subset used_vars (Efun fds e).
-  Proof.
-    intros; intros x Hx.
-    destruct Hx; [left; auto|].
-    split_var_in_fundefs x fds Hfds.
-    left; constructor; now apply name_in_fundefs_bound_var_fundefs.
-    right; constructor; auto.
-  Qed.
+  Proof. intros; normalize_used_vars; auto with Ensembles_DB. Qed.
 
   Lemma used_vars_fundefs_Efun_Included: forall fds e,
     used_vars_fundefs fds \subset used_vars (Efun fds e).
-  Proof.
-    intros; intros x Hx.
-    destruct Hx; [left; auto|].
-    right; now apply Free_Efun2.
-  Qed.
+  Proof. intros; normalize_used_vars; auto with Ensembles_DB. Qed.
 
   Lemma uncurry_step_s_nondecreasing_mut :
     let P := (fun e s m e1 s1 m1 => s \subset s1) in
@@ -2417,14 +1894,20 @@ Section uncurry_correct.
 
   Lemma Union_Included_lr : forall {A} (S1 S2 S3 : _ A),
     S1 :|: S2 \subset S3 -> S1 \subset S3 /\ S2 \subset S3.
-  Proof.
-    intros; split; [eapply Union_Included_l|eapply Union_Included_r]; eauto.
-  Qed.
+  Proof. intros; split; [eapply Union_Included_l|eapply Union_Included_r]; eauto. Qed.
 
   Local Ltac destruct_Union_Included :=
     repeat match goal with
       [ H : _ :|: _ \subset _ |- _ ] => apply Union_Included_lr in H; destruct H
     end.
+
+  Local Ltac inv_all :=
+    repeat match goal with
+    | [ H : Ensembles.In var _ _ |- _ ] => inv H
+    | [ H : List.In _ _ |- _ ] => inv H
+    | [ H : (_, _) = (_, _) |- _ ] => inv H
+    end;
+    eauto with Ensembles_DB.
 
   Lemma uncurry_step_preserves_used_vars_mut :
     let P := (fun e s m e1 s1 m1 => used_vars e \subset s -> used_vars e1 \subset s1) in
@@ -3282,10 +2765,13 @@ Section uncurry_correct.
       [ intros k .. | intros f' k' e' | intros f' k' e' | intros f' k' e' | intros f' k' e' ];
       intros Hunique Hunique1 Hused Hused1 rho rho1 Henv.
     - (* uncurry_constr *)
-      eapply preord_exp_const_compat; try eassumption.
+      eapply preord_exp_const_compat.
       + unfold preord_env_P in Henv.
         apply Forall2_same.
-        intros a Hin. (* apply Henv.
+        intros a Hin.
+        Check preord_var_env.
+        SearchAbout inclusion.
+        (* apply Henv.
         now apply Free_Econstr1. *) admit.
       + intros args1 args2 Hargs.
         apply IH; inv Hunique; inv Hunique1; auto.
